src/PlutusIR/Semantics/Static/Typing/drop_context.v
@@ -1,0 +1,449 @@
+Require Import PlutusCert.PlutusIR.
+Require Import PlutusCert.Util.List.
+
+Require Export PlutusCert.PlutusIR.Semantics.Static.Auxiliary.
+Require Export PlutusCert.PlutusIR.Semantics.Static.Context.
+Require Export PlutusCert.PlutusIR.Semantics.Static.Typing.Typing.
+Require Export PlutusCert.PlutusIR.Semantics.Static.Kinding.Kinding.
+Require Export PlutusCert.PlutusIR.Semantics.Static.TypeSubstitution.
+Require Import PlutusCert.PlutusIR.Analysis.BoundVars.
+Require Export PlutusCert.PlutusIR.Analysis.FreeVars.
+
+From PlutusCert Require Import util Util.
+
+Require Import Coq.Program.Equality.
+Import Coq.Lists.List.
+Import ListNotations.
+Import Coq.Strings.String.
+Local Open Scope string_scope.
+Open Scope list_scope.
+
+(* ************* drop_ty_var ************* *)
+
+Lemma drop_ty_var__inclusion X Γ :
+  List.inclusion (drop_ty_var X Γ) Γ.
+Proof.
+  unfold List.inclusion.
+  intros x v Hl.
+  induction Γ.
+  - inversion Hl.
+  - simpl.
+    destruct a as [a1 a2].
+    (* TODO: destr_eqb_eq tactic *)
+    destruct (string_dec a1 x); subst.
+    + rewrite String.eqb_refl.
+      f_equal.
+      (* Suppose X in a2. Then by Hl
+        we have that a2 <> v
+
+        But then by drop_ty_var, all keys "x" will be removed from Hl,
+        hence contradiction, because then it would have been None.
+
+        Hence we must have X not in a2.
+        Then by Hl we have lookup x ((x, a2)::...) = Some v => a2 = v
+      *)
+      admit.
+    + rewrite <- String.eqb_neq in n.
+      rewrite n.
+      (* a1 <> x
+        lookup x (drop ((a1, a2)::Γ) = Some v)
+        Well, it is not the first one (a1), and the result is Some v.
+        Hence we must have lookup x (drop Γ) = Some v. (possibly with even smaller Gamma, if a2 contains X)
+        since drop Γ is a subset of Γ, we must have then also lookup x Γ = Some v.
+      *)
+
+Admitted.
+
+Lemma drop_ty_var__inclusion_preserving : forall X Γ Γ',
+    List.inclusion Γ Γ' -> List.inclusion (drop_ty_var X Γ) (drop_ty_var X Γ').
+Proof.
+intros X Γ Γ' Hincl.
+unfold List.inclusion in Hincl.
+unfold List.inclusion.
+intros x v Hl.
+(* by contradiction:
+  Suppose lookup x (drop_ty_var X Γ') = None
+
+    By drop_ty_var__inclusion,
+      we have lookup x Γ' = Some v.
+
+      then
+        (x, v) in Gamma' and X in v (not possible by Hl)
+      OR
+        (x, v') in Gamma' and X in v', then also (x, v) gets removed
+
+        But if this (x, v') occured to the right of (x, v), then still (x, v) in Gamma
+        If it occurred to the left, we would have had
+        lookup x Γ' = Some v' with v <> v'. Contradiction.
+*)
+Admitted.
+
+Lemma drop_ty_var__lookup_some : forall X Γ x T,
+    lookup x (drop_ty_var X Γ) = Some T ->
+    exists T', lookup x Γ = Some T'.
+(* Drop ty var cannot remove anything, so we cannot get None
+  we are not guaranteed to get the same, as (x, S(X)) could be dropped and in front of (x, T).
+*)
+Admitted.
+
+(* Drop Δ *)
+
+Lemma drop_Δ_nil : forall Δ,
+    drop_Δ Δ nil = Δ.
+Proof.
+  intros Δ.
+  unfold drop_Δ.
+  induction Δ.
+  - simpl. reflexivity.
+  - simpl. f_equal.
+    auto.
+Qed.
+
+From Coq Require Import Bool.
+
+Lemma drop_Δ__weaken : forall Δ b bs,
+  drop_Δ Δ (b::bs) = drop_Δ (binds_Delta b ++ Δ) (b::bs).
+Proof.
+  intros Δ b bs; unfold drop_Δ.
+  induction b.
+  - simpl. reflexivity.
+  - simpl. destruct t.
+    unfold drop_Δ'.
+    remember (fun x : string * kind => _) as f.
+
+    assert (Hf_nil: filter f [(b, k)] = []).
+    {
+      subst; simpl.
+      assert (Hin: (inb_string b (btvbs (TypeBind (TyVarDecl b k) t0 :: bs))) = true).
+      {
+        unfold btvbs; simpl.
+        rewrite inb_string_true_iff.
+        apply in_eq.
+      }
+      rewrite Hin; auto.
+    }
+    assert (Hf_app: filter f Δ = filter f [(b, k)] ++ filter f Δ).
+    {
+      rewrite Hf_nil.
+      rewrite app_nil_l.
+      reflexivity.
+    }
+    rewrite Hf_app.
+    rewrite filter_app; auto.
+  - simpl. destruct d. destruct t.
+    unfold drop_Δ'.
+    remember (fun x : string * kind => _) as f.
+    assert (Hf_nil: filter f [(b0, k)] = []).
+    {
+      subst; simpl.
+      assert (Hin: (inb_string b0 (btvbs (DatatypeBind (Datatype (TyVarDecl b0 k) l b l0) :: bs))) = true).
+      {
+        unfold btvbs; simpl.
+        rewrite inb_string_true_iff.
+        apply in_eq.
+      }
+      rewrite Hin; auto.
+    }
+    assert (Hf_app: filter f Δ = filter f [(b0, k)] ++ filter f Δ).
+    {
+      rewrite Hf_nil.
+      rewrite app_nil_l.
+      reflexivity.
+    }
+    rewrite Hf_app.
+    rewrite filter_app; auto.
+Qed.
+
+
+Lemma drop_Δ__unfold : forall Δ b bs,
+  drop_Δ Δ (b::bs) = drop_Δ (drop_Δ Δ bs) [b].
+Proof.
+  intros Δ b bs.
+  induction Δ.
+  - simpl. reflexivity.
+  - simpl.
+    destruct (inb_string (fst a) (btvbs (b :: bs))) eqn:Heqn1.
+    + (* a = b or In a (btvb bs)*)
+      simpl.
+      destruct (inb_string (fst a) (btvbs bs)) eqn:Heqn2.
+      * (* a in bs *)
+        simpl.
+        apply IHΔ.
+      * (* a notin bs, so then a = b*)
+        simpl.
+        assert (inb_string (fst a) (btvbs [b]) = true ).
+        {
+          rewrite btvbs_cons in Heqn1.
+          rewrite inb_string_true_iff in Heqn1.
+          rewrite in_app_iff in Heqn1. 
+          destruct Heqn1 as [Heqn1 | Heqn1].
+          - rewrite <- inb_string_true_iff in Heqn1.
+            unfold btvbs; simpl.
+            rewrite app_nil_r.
+            assumption.
+          - rewrite <- inb_string_true_iff in Heqn1.
+            rewrite Heqn1 in Heqn2.
+            inversion Heqn2.
+        }
+        simpl.
+        rewrite H.
+        simpl.
+        apply IHΔ.
+    + (* ~ In a (btvbs (b :: bs))*)
+      assert (
+        (inb_string (fst a) (btvbs bs)) = false).
+      {
+        rewrite btvbs_cons in Heqn1.
+        rewrite inb_string_false_iff in Heqn1.
+        rewrite not_in_app in Heqn1.
+        destruct Heqn1 as [_ Heqn1].
+        rewrite <- inb_string_false_iff in Heqn1.
+        assumption.
+      }
+      rewrite H.
+      simpl.
+      assert ((inb_string (fst a) (btvbs [b])) = false).
+      {
+        rewrite btvbs_cons in Heqn1.
+        rewrite inb_string_false_iff in Heqn1.
+        rewrite not_in_app in Heqn1.
+        destruct Heqn1 as [Heqn1 _].
+        rewrite <- inb_string_false_iff in Heqn1.
+        unfold btvbs. simpl.
+        rewrite app_nil_r.
+        assumption.
+      }
+      rewrite H0; simpl.
+      f_equal.
+      apply IHΔ.
+Qed.
+
+Lemma drop_Δ_nil__kinding : forall Δ T K,
+    drop_Δ Δ nil |-* T : K -> Δ |-* T : K.
+Proof.
+  intros.
+  rewrite drop_Δ_nil in H.
+  assumption.
+Qed.
+    
+  Lemma drop_Δ'__lookup_None : forall Δ xs x,
+    In x (xs) -> lookup x (drop_Δ' Δ xs) = None.
+  Proof.
+    intros Δ xs x Hbtvbs.
+    induction Δ; simpl.
+    - reflexivity.
+    - destruct a as [a1 a2]; simpl.
+      destruct (negb (inb_string a1 (xs))) eqn:Heqn.
+      + destruct (string_dec a1 x).
+        * subst.
+          exfalso.
+          rewrite negb_true_iff in Heqn.
+          rewrite inb_string_false_iff in Heqn.
+          contradiction.
+        * simpl.
+          rewrite <- String.eqb_neq in n.
+          rewrite n.
+          exact IHΔ.
+    + assumption.
+  Qed.
+
+  Lemma drop_Δ__lookup_None : forall Δ bs x,
+    In x (BoundVars.btvbs bs) -> lookup x (drop_Δ Δ bs) = None.
+  Proof.
+    intros.
+    unfold drop_Δ.
+    eapply drop_Δ'__lookup_None.
+    assumption.
+  Qed.
+
+  Lemma dropped_not_in_drop_Δ' : forall Δ xs x,
+    In x xs ->
+    ~ In x (map fst (drop_Δ' Δ xs)).
+  Proof.
+    intros Δ xs x Hin.
+    apply drop_Δ'__lookup_None with (Δ := Δ) in Hin.
+    apply lookup__not_in in Hin.
+    assumption.
+  Qed.
+
+   Lemma lookup_None__drop_Δ' : forall Δ xs x,
+    ~ In x xs ->
+    lookup x (drop_Δ' Δ xs) = lookup x Δ.
+  Proof.
+    intros Δ xs x HnotBtvb.
+    induction Δ; simpl.
+    - reflexivity.
+    - destruct a as [a1 a2]; simpl.
+      destruct ((inb_string a1 xs)) eqn:Heqn; simpl.
+      + destruct (string_dec a1 x).
+        * subst.
+          rewrite inb_string_true_iff in Heqn.
+          contradiction.
+        * rewrite <- String.eqb_neq in n.
+          rewrite n.
+          rewrite IHΔ; auto.
+      + simpl.
+        destruct (string_dec a1 x).
+        * subst.
+          rewrite String.eqb_refl.
+          reflexivity.
+        * rewrite <- String.eqb_neq in n.
+          rewrite n.
+          rewrite IHΔ; auto. 
+  Qed.
+
+  Lemma lookup_None__drop_Δ : forall Δ bs x,
+    ~ In x (BoundVars.btvbs bs) ->
+    lookup x (drop_Δ Δ bs) = lookup x Δ.
+  Proof.
+    intros.
+    unfold drop_Δ.
+    eapply lookup_None__drop_Δ'.
+    assumption.
+  Qed.
+
+  Lemma lookup_Some__drop_Δ'_no_xs : forall Δ xs x K,
+    lookup x (drop_Δ' Δ xs) = Some K ->
+    ~ In x xs.
+  Proof.
+    intros Δ xs x K Hl.
+    induction Δ; simpl in *.
+    - inversion Hl.
+    - destruct a as [a1 a2]; simpl in *.
+      destruct (inb_string a1 xs) eqn:Heqn; simpl in *.
+      + destruct (string_dec a1 x).
+        * apply IHΔ.
+          assumption.
+        * subst.
+          apply IHΔ.
+          exact Hl.
+      + simpl in Hl.
+        destruct (string_dec a1 x).
+        * subst.
+          rewrite inb_string_false_iff in Heqn.
+          assumption.
+        * rewrite <- String.eqb_neq in n.
+          rewrite n in Hl.
+          apply IHΔ.
+          assumption.
+  Qed.
+
+  Lemma lookup_Some__drop_Δ_no_btvbs : forall Δ bs x K,
+    lookup x (drop_Δ Δ bs) = Some K ->
+    ~ In x (BoundVars.btvbs bs).
+  Proof.
+    intros.
+    unfold drop_Δ.
+    eapply lookup_Some__drop_Δ'_no_xs; eauto.
+  Qed.
+
+  Lemma drop_Δ'__inclusion : forall Δ xs,
+    List.inclusion (drop_Δ' Δ xs) Δ.
+  Proof.
+    intros.
+    induction Δ; simpl.
+    - unfold List.inclusion; auto.
+    - destruct a as [a1 a2].
+      destruct (inb_string (fst (a1, a2)) xs) eqn:Heqn; simpl in *.
+      + unfold inclusion.
+        intros x v Hl.
+        destruct (string_dec a1 x).
+        * subst.
+          exfalso.
+          rewrite inb_string_true_iff in Heqn.
+          eapply drop_Δ'__lookup_None in Heqn.
+          rewrite Hl in Heqn.
+          inversion Heqn.
+        * simpl.
+          rewrite <- String.eqb_neq in n.
+          rewrite n.
+          apply IHΔ.
+          assumption.
+      + unfold inclusion.
+        intros x v Hl.
+        destruct (string_dec a1 x).
+        * subst.
+          inversion Hl.
+          rewrite String.eqb_refl.
+          simpl.
+          rewrite String.eqb_refl.
+          reflexivity.
+        * simpl.
+          rewrite <- String.eqb_neq in n.
+          rewrite n.
+          apply IHΔ.
+          simpl in Hl.
+          rewrite n in Hl.
+          assumption.
+  Qed.
+
+  Lemma drop_Δ__inclusion : forall Δ bs,
+    List.inclusion (drop_Δ Δ bs) Δ.
+  Proof.
+    intros.
+    unfold drop_Δ.
+    eapply drop_Δ'__inclusion.
+  Qed.
+
+
+Lemma drop_Δ_cons__inclusion : forall Δ b bs,
+    List.inclusion (drop_Δ Δ (b::bs)) (drop_Δ (binds_Delta b ++ Δ) bs).
+Proof.
+  intros Δ b bs.
+  assert (Hweaken: drop_Δ Δ (b::bs) = drop_Δ (binds_Delta b ++ Δ) (b::bs)).
+  {
+    apply drop_Δ__weaken.
+  }
+  rewrite Hweaken; clear Hweaken.
+  assert (Hunfold: drop_Δ (binds_Delta b ++ Δ) (b::bs) = drop_Δ (drop_Δ (binds_Delta b ++ Δ) bs) [b]).
+  {
+    apply drop_Δ__unfold.
+  }
+  rewrite Hunfold; clear Hunfold.
+  apply drop_Δ__inclusion.
+Qed.
+
+  Lemma drop_Δ'__preserves__inclusion : forall Δ Δ' xs,
+      List.inclusion Δ Δ' ->
+      List.inclusion (drop_Δ' Δ xs) (drop_Δ' Δ' xs).
+  Proof.
+    intros Δ Δ' xs Hincl.
+    unfold inclusion in *.
+    intros x v Hl.
+    assert (lookup x Δ' = Some v).
+    {
+      apply drop_Δ'__inclusion in Hl.
+      apply Hincl in Hl.
+      assumption.
+    }
+    assert ( ~ In x xs).
+    {
+      eapply lookup_Some__drop_Δ'_no_xs; eauto.
+    }
+
+    induction Δ'.
+    - inversion H.
+    - eapply lookup_None__drop_Δ' in H0; eauto.
+      rewrite H0.
+      assumption.
+  Qed.
+
+  Lemma drop_Δ__preserves__inclusion : forall Δ Δ' bs,
+      List.inclusion Δ Δ' ->
+      List.inclusion (drop_Δ Δ bs) (drop_Δ Δ' bs).
+  Proof.
+    intros.
+    unfold drop_Δ.
+    eapply drop_Δ'__preserves__inclusion.
+    assumption.
+  Qed.
+
+Lemma btvbs_eq__drop_Δ_eq : forall Δ bs bs',
+  btvbs bs = btvbs bs' ->
+  drop_Δ Δ bs = drop_Δ Δ bs'.
+Proof.
+  intros Δ bs bs' Hbtvbs.
+  unfold drop_Δ.
+  rewrite Hbtvbs.
+  reflexivity.
+Qed.
